imper/Dijkstra.ml
@@ -1,7 +1,6 @@
 module type Ordered =
 sig 
    type t
-   type t
    val le : t -> t -> bool
 end 
 
@@ -17,34 +16,44 @@ end
 
 type len = Finite of int | Infinite
 
-module NextNode : Ordered with type t = int * int
+module NextNode = (* Ordered with type t = int * int *)
 struct
    type t = int * int
-   let le (_,d1) (_,d2) -> (d1 <= d2)
+   let le : t -> t -> bool =
+     fun (_,d1) (_,d2) -> (d1 <= d2)
 end
 
-module Dijkstra (Heap:HeapSig with module Element = NextNode) = 
+module type HeapNextNodeSig =
+sig
+  type heap
+  val create : unit -> heap
+  val is_empty : heap -> bool
+  val push : NextNode.t -> heap -> unit
+  val pop : heap -> NextNode.t
+end
+
+module Dijkstra (Heap:HeapNextNodeSig) = (* Heap : HeapSig with module Element = NextNode *)
 struct 
-   let shortest_path g a b = 
+   let shortest_path g s e = 
       let n = Array.length g in
-      let b = Array.make n Inf in
+      let b = Array.make n Infinite in
       let t = Array.make n false in
       let h = Heap.create() in
-      b.(a) <- Finite 0;
-      Heap.push (a,0) h;
+      b.(s) <- Finite 0;
+      Heap.push (s,0) h;
       while not (Heap.is_empty h) do
          let (x,dx) = Heap.pop h in
          if not t.(x) then begin
             t.(x) <- true;
-            let udpate (y,w) =
+            let update (y,w) =
               let dy = dx + w in
                  if (match b.(y) with | Finite d -> dy < d
-                                      | _ -> True) then 
+                                      | _ -> true) then 
                     (b.(y) <- Finite dy; 
-                     Heap.push h (y,dy))
+                     Heap.push (y,dy) h)
                in
             List.iter update g.(x);
          end;
       done;
-      dist.(b)
+      b.(e)
 end
