imper/old_dijkstra.ml
@@ -1,3 +1,69 @@
+module type Ordered =
+sig 
+   type t
+   val le : t -> t -> bool
+end 
+
+module type HeapSig =
+sig
+  module Element : Ordered
+  type heap
+  val create : unit -> heap
+  val is_empty : heap -> bool
+  val push : Element.t -> heap -> unit
+  val pop : heap -> Element.t 
+end
+
+type len = Finite of int | Infinite
+
+module NextNode  =
+struct
+   type t = int * int
+   let le : t -> t -> bool =
+     fun (_,d1) (_,d2) -> (d1 <= d2)
+end
+
+(*
+module type OrderedPairInt = Ordered with type t = int * int
+
+module NextNode : OrderedPairInt =
+struct
+   type t = int * int
+   let le (_,d1) (_,d2) = (d1 <= d2)
+end
+
+module type HeapNextNodeSig = HeapSig with module Element = NextNode
+
+module Dijkstra (Heap:HeapNextNodeSig) = 
+struct 
+   let shortest_path g s e = 
+      let n = Array.length g in
+      let b = Array.make n Infinite in
+      let t = Array.make n false in
+      let h = Heap.create() in
+      b.(s) <- Finite 0;
+      Heap.push (s,0) h;
+      while not (Heap.is_empty h) do
+         let (x,dx) = Heap.pop h in
+         if not t.(x) then begin
+            t.(x) <- true;
+            let update (y,w) =
+              let dy = dx + w in
+                 if (match b.(y) with | Finite d -> dy < d
+                                      | _ -> true) then 
+                    (b.(y) <- Finite dy; 
+                     Heap.push (y,dy) h)
+               in
+            List.iter update g.(x);
+         end;
+      done;
+      b.(e)
+end
+*)
+
+
+
+
 Definition source_ok B :=
   B\(a) = 0.
 
