imper/Dijkstra_proof.v
@@ -2,6 +2,12 @@ Set Implicit Arguments.
 Require Import CFLib Dijkstra_ml.
 Open Scope comp_scope.
 
+(*
+Module Type MLOrderedPairInt :=
+  MLOrdered with Definition t := (int*int)%type.
+Module MLNextNode' :  MLOrdered with Definition t := (int*int)%type.
+*)
+
 (*************************************************************)
 
 
@@ -12,22 +18,22 @@ Definition Min A (f:A->int) (P:A->Prop) :=
                  /\ (forall x, P x -> n <= f x)).
 
 Definition MinBar A (f:A->int) (P:A->Prop) :=  
-  If (exists x, P x) Then Finite(Min f P) Else Infinite.
+  If (exists x, P x) then Finite(Min f P) else Infinite.
 
-Lemma MinBar_Infinite : forall A (f:A->int) P,
+Lemma MinBar_Infinite : forall A (f:A->int) (P:A->Prop),
   (forall x, ~ P x) -> MinBar f P = Infinite.
 Proof. Admitted.
 
-Lemma MinBar_Finite : forall A x (f:A->int) P,
+Lemma MinBar_Finite : forall A x (f:A->int) (P:A->Prop),
   P x -> (forall y, f x <= f y) ->
   MinBar f P = Finite (f x).
 Proof. Admitted.
 
-Lemma MinBar_Finite_inv : forall A n x (f:A->int) P,
+Lemma MinBar_Finite_inv : forall A n x (f:A->int) (P:A->Prop),
   MinBar f P = Finite n -> P x -> n <= f x.
 Proof. Admitted.
 
-Lemma MinBar_Infinite_inv : forall A x (f:A->int) P,
+Lemma MinBar_Infinite_inv : forall A x (f:A->int) (P:A->Prop),
   MinBar f P = Infinite -> ~ P x.
 Proof. Admitted.
 
@@ -50,16 +56,16 @@ Definition nonnegative_edges (g:graph int) :=
 
 Definition path A := list (int*int*A).
 
-Inductive is_path A (g:graph A) : int -> int -> Prop :=
+Inductive is_path A (g:graph A) : int -> int -> path A -> Prop :=
   | is_path_nil : forall x, 
-      is_path nil
+      is_path g x x nil
   | is_path_cons : forall x y z w p,
       is_path g x y p ->
       has_edge g y z w ->
       is_path g x z ((y,z,w)::p).
 
 Definition weight (p:path int) :=
-  nosimpl (fold_left (fun e acc => let '(_,_,w) := e in w+acc) 0).
+  nosimpl (fold_right (fun e acc => let '(_,_,w) := e in w+acc) 0 p).
 
 Definition dist (g:graph int) x y :=  
   MinBar weight (is_path g x y).
@@ -71,7 +77,7 @@ Proof. auto. Qed.
 
 Lemma weight_cons : forall (p:path int) x y w, 
   weight ((x,y,w)::p) = w + weight p.
-Proof. unfold weight; rew_list~. Qed.
+Proof. intros. unfold weight. rew_list~. Qed.
 
 (*-----------------------------------------------------------*)
 
@@ -79,7 +85,7 @@ Parameter range : int -> int -> set int.
 
 Definition GraphAdjList (G:graph int) (g:loc) :=
   Hexists N, g ~> Array Id N
-         \* [nodes G = range 0 (size N)]
+         \* [nodes G = range 0 (LibArray.length N)]
          \* [forall_ x \in (nodes G), forall y w, 
                Mem (y,w) (N\(x)) = has_edge G x y w].
 
@@ -97,7 +103,7 @@ Global Instance le_inst : Le T.
 Global Instance le_order : Le_total_order.
 
 Parameter le_spec : Spec le (x:t) (y:t) |R>> forall Y X, 
-  keep R (x ~> S X \* y ~> S Y) (\= isTrue (LibOrder.le X Y)).
+  keep R (x ~> S X \* y ~> S Y) (\= istrue (LibOrder.le X Y)).
 
 Hint Extern 1 (RegisterSpec le) => Provide le_spec.
 
@@ -115,11 +121,11 @@ Definition is_min_of `{Le A} (E:multiset A) (X:A) :=
 
 Module Type HeapSigSpec.
 
-Declare Module H : MLHeap.
+Declare Module H : MLHeapSig.
 Declare Module OS : OrderedSigSpec with Module O := H.MLElement.
 Import H MLElement OS. 
 
-Parameter Heap : htype (multiset T) heap.
+Parameter Heap : htype T t -> htype (multiset T) heap.
 
 Parameter create_spec :
   Spec create () |R>> 
@@ -127,39 +133,41 @@ Parameter create_spec :
 
 Parameter is_empty_spec : 
   Spec is_empty (h:heap) |R>> forall E,
-    keep R (h ~> Heap S E) (\= isTrue (E = \{})).
+    keep R (h ~> Heap S E) (\= istrue (E = \{})).
 
 Parameter push_spec : 
   Spec push (x:t) (h:heap) |R>> forall E X,
-    R (h ~> Heap S E \* x ~> S X) (# h ~> Heap (\{X} \u E)).
+    R (h ~> Heap S E \* x ~> S X) (# h ~> Heap S (\{X} \u E)).
 
 Parameter pop_spec : 
   Spec pop (h:heap) |R>> forall E,
     R (h ~> Heap S E) (fun x => Hexists X F, 
-      [is_min_of E X] \* [E = \{X} \u F] \* x ~> S X \* h ~> Heap F).
+      [is_min_of E X] \* [E = \{X} \u F] \* x ~> S X \* h ~> Heap S F).
 
 End HeapSigSpec.
 
 
 (*************************************************************)
 
-Module NextNodeSpec :> OrderedSigSpec with Module O := NextNode.
-Module O := NextNode.
+Module NextNodeSpec <: OrderedSigSpec with Module O := MLNextNode.
+Module O := MLNextNode.
 Import O.
-Definition T : Type := int*int.
+Definition T : Type := (int*int)%type.
 Definition S : htype T t := Id.
 
 Global Instance le_inst : Le T.
-  exists (fun p1 p2 => snd p1 <= snd p2).
+Proof.
+  constructor.
+  exact (fun (p1 p2 : int*int) => snd p1 <= snd p2).
 Defined.
   
 Global Instance le_order : Le_total_order.
-Admitted.
+Admitted. (* todo :order prod *)
 
 Lemma le_spec : Spec le (x:t) (y:t) |R>> forall Y X, 
-  keep R (x ~> S X \* y ~> S Y) (\= isTrue (LibOrder.le X Y)).
+  keep R (x ~> S X \* y ~> S Y) (\= istrue (LibOrder.le X Y)).
 Proof.
-Qed.
+Admitted.
 
 Hint Extern 1 (RegisterSpec le) => Provide le_spec.
 
@@ -167,37 +175,50 @@ End NextNodeSpec.
 
 (*************************************************************)
 
+Global Instance len_inhab : Inhab len.
+Proof. constructor. exact Infinite. Qed.
+
+
+(*************************************************************)
+Require Import LibArray LibMap.
+
 Module DijkstraSpec.
-Declare Module Heap : MLHeapSig with module MLElement = MLNextNode.
+Declare Module Heap : MLHeapSig with Module MLElement := MLNextNode.
 Import NextNodeSpec.
 
-Implicit Types T : array int.
-Implicit Types B : array int.
-Implicit Types H : set int.
+Implicit Types T : array bool.
+Implicit Types B : array len.
+Implicit Types H : set (int*int).
+Implicit Types p : path int.
 
 Section Invariants.
-Variables (G:graph int) (a:int).
+Variables (G:graph int) (s:int).
 
 (*-----------------------------------------------------------*)
 
+Global Instance test : BagRead int Type (array bool).
+Proof. constructor. exact (fun t i => read t i = true). Defined.
+Global Instance test' : BagRead int Prop (array bool).
+Proof. constructor. exact (fun t i => read t i = true). Defined.
+
 Record inv T B H reach : Prop :=
-  { source_ok     : B\(a) = 0;
-    treated_ok    : forall v, T\(v) -> B\(v) = dist G a v;
-    untreated_ok  : forall v, ~ T\(v) -> v <> a -> 
-                      B\(v) = MinBar weight reach;
-    heap_correct  : forall v d, ~ T\(v) -> v <> a -> (v,d) \in H -> 
+  { source_ok     : B\(s) = Finite 0;
+    treated_ok    : forall v, T\(v) -> B\(v) = dist G s v;
+    untreated_ok  : forall v, ~ T\(v) -> v <> s -> 
+                      B\(v) = MinBar weight (reach v);
+    heap_correct  : forall v d, ~ T\(v) -> v <> s -> (v,d) \in H -> 
                       exists p, reach v p /\ weight p = d;
     heap_complete : forall v p, reach v p -> 
                       exists d, (v,d) \in H /\ d <= weight p }.  
 
 Definition enters T v p := 
-  exists q y w, is_path G a y q 
+  exists q y w, is_path G s y q 
              /\ has_edge G y v w
              /\ T\(y)
              /\ ~ T\(v).
   
 Definition enters_via x L v p :=
-  exists q w, p = (x,v,w)::q /\ is_path G a x q /\ Mem (v,w) L.
+  exists q w, p = (x,v,w)::q /\ is_path G s x q /\ Mem (v,w) L.
 
 Definition new_enters x L T v p :=
   enters T v p \/ enters_via x L v p.
@@ -212,17 +233,18 @@ Admitted.
 Lemma new_enters_inv : forall x L T v p y w,
   new_enters x ((y,w)::L) T v p -> 
       new_enters x L T v p 
-   \/ exists q, p = (x,y,w)::q /\ is_path G a x q.
+   \/ exists q, p = (x,y,w)::q /\ is_path G s x q.
 Proof.
 Admitted.
 
-Lemma enters_step : forall T x v p, ~ T\(x) ->
-  enters (T\(x:=true)) v p = (enters T v p \/ enters_via x (N\(x)) v p).
+Lemma enters_step : forall L T x v p, ~ T\(x) ->
+  (forall y w, Mem (y,w) L <-> (x,y,w) \in edges G) ->
+  enters (T\(x:=true)) v p = (enters T v p \/ enters_via x L v p).
 Proof.
 Admitted.
 
-Lemma enters_shorter : forall T y p, 
-  ~ T\(v) -> is_path G a y p ->
+Lemma enters_shorter : forall T v y p, 
+  ~ T\(v) -> is_path G s y p ->
   exists z q, enters T z q /\ weight q <= weight p.
 Proof.
 Admitted.
@@ -230,7 +252,7 @@ Admitted.
 Lemma enters_best : forall T x p,
   ~ T\(x) -> enters T x p ->
   (forall y q, enters T y q -> weight p <= weight q) ->
-  dist G a x = Fin (weight p).
+  dist G s x = Finite (weight p).
 Proof.
 Admitted.
 
